Prove global variable allocation for example

new/golang/theory/globals.v
@@ -21,41 +21,16 @@ Section definitions.
 Context `{ffi_sem: ffi_semantics} `{!ffi_interp ffi} `{!heapGS Σ}.
 Context `{!goGlobalsGS Σ}.
 
-Definition is_global_addr_def (pkg_name var_name : string) (addr : loc) : iProp Σ :=
-  ∃ γpkg,
-  pkg_name ↪[go_package_gname_name]□ γpkg ∗
-  var_name ↪[γpkg]□ addr.
-
-Definition own_unused_packages_def (used_package_names : gset string) : iProp Σ :=
-  ∃ m,
-    ghost_map_auth go_package_gname_name 1%Qp m ∗
-    ⌜ dom m = used_package_names ⌝.
-
-Definition own_unused_vars_def (pkg_name : string) (used_var_names : gset string) : iProp Σ :=
-  ∃ γpkg (m : gmap string loc),
-  "#Hγpkg" ∷ pkg_name ↪[go_package_gname_name]□ γpkg ∗
-  "Hpkg_auth" ∷ ghost_map_auth γpkg (1/2)%Qp m ∗
-  "%Hused_vars_dom" ∷ ⌜ dom m = used_var_names ⌝.
-
-Local Definition encode_var_name (pkg_name var_name : string) : string :=
-  pkg_name +:+ " " +:+ var_name.
-
-Local Definition is_valid_package_name (pkg_name : string) : Prop :=
+Local Definition is_valid_package_name_prop (pkg_name : string) : Prop :=
   " "%char ∉ (String.list_ascii_of_string pkg_name).
 
-Lemma encode_var_name_inj pkg_name1 pkg_name2 var_name1 var_name2 :
-  is_valid_package_name pkg_name1 →
-  is_valid_package_name pkg_name2 →
-  encode_var_name pkg_name1 var_name1 = encode_var_name pkg_name2 var_name2 →
-  pkg_name1 = pkg_name2 ∧ var_name1 = var_name2.
-Proof.
-Admitted.
+Fixpoint is_valid_package_name (pkg_name : string) : bool :=
+  match pkg_name with
+  | EmptyString => true
+  | String a s => negb (Ascii.eqb a " "%char) && is_valid_package_name s
+  end.
 
-Lemma encode_var_name_package_name_ne pkg_name' pkg_name var_name :
-  is_valid_package_name pkg_name' →
-  pkg_name' ≠ encode_var_name pkg_name var_name.
-Proof.
-Admitted.
+Local Notation encode_var_name := (globals.globals.encode_var_name).
 
 Definition own_globals_inv : iProp Σ :=
   ∃ g (package_gnames : gmap string gname),
@@ -81,29 +56,80 @@ Definition own_globals_inv : iProp Σ :=
                                     end ⌝
 .
 
-Definition is_globals_inv : iProp Σ :=
+Local Definition is_globals_inv : iProp Σ :=
   inv nroot own_globals_inv.
 
-Lemma wp_globals_put pkg_name var_name used_var_names (addr : loc) :
-  var_name ∉ used_var_names →
-  is_valid_package_name pkg_name →
-  {{{ is_globals_inv ∗ own_unused_vars_def pkg_name used_var_names }}}
-    globals.put #(encode_var_name pkg_name var_name) #addr
+Definition is_global_addr_def (var_id : string * string) (addr : loc) : iProp Σ :=
+  let (pkg_name, var_name) := var_id in
+  ∃ γpkg,
+    is_globals_inv ∗
+    pkg_name ↪[go_package_gname_name]□ γpkg ∗
+    var_name ↪[γpkg]□ addr.
+Program Definition is_global_addr := unseal (_:seal (@is_global_addr_def)). Obligation 1. by eexists. Qed.
+Definition is_global_addr_unseal : is_global_addr = _ := seal_eq _.
+
+Definition own_unused_packages_def (used_package_names : gset string) : iProp Σ :=
+  ∃ m,
+    is_globals_inv ∗
+    ghost_map_auth go_package_gname_name 1%Qp m ∗
+    ⌜ dom m = used_package_names ⌝.
+Program Definition own_unused_packages := unseal (_:seal (@own_unused_packages_def)). Obligation 1. by eexists. Qed.
+Definition own_unused_packages_unseal : own_unused_packages = _ := seal_eq _.
+
+Definition own_unused_vars_def (pkg_name : string) (used_var_names : gset string) : iProp Σ :=
+  ∃ γpkg (m : gmap string loc),
+    "#Hinv" ∷ is_globals_inv ∗
+    "#Hγpkg" ∷ pkg_name ↪[go_package_gname_name]□ γpkg ∗
+    "Hpkg_auth" ∷ ghost_map_auth γpkg (1/2)%Qp m ∗
+    "%Hused_vars_dom" ∷ ⌜ dom m = used_var_names ⌝.
+Program Definition own_unused_vars := unseal (_:seal (@own_unused_vars_def)). Obligation 1. by eexists. Qed.
+Definition own_unused_vars_unseal : own_unused_vars = _ := seal_eq _.
+
+Local Ltac unseal := rewrite
+  ?is_global_addr_unseal
+  ?own_unused_packages_unseal
+  ?own_unused_vars_unseal.
+
+Global Instance is_global_addr_persistent x a:
+  Persistent (is_global_addr x a).
+Proof. unseal. destruct x. apply _. Qed.
+
+Lemma encode_var_name_inj pkg_name1 pkg_name2 var_name1 var_name2 :
+  is_valid_package_name pkg_name1 →
+  is_valid_package_name pkg_name2 →
+  encode_var_name pkg_name1 var_name1 = encode_var_name pkg_name2 var_name2 →
+  pkg_name1 = pkg_name2 ∧ var_name1 = var_name2.
+Proof.
+Admitted.
+
+Lemma encode_var_name_package_name_ne pkg_name' pkg_name var_name :
+  is_valid_package_name pkg_name' →
+  pkg_name' ≠ encode_var_name pkg_name var_name.
+Proof.
+Admitted.
+
+
+Lemma wp_globals_put var_id used_var_names (addr : loc) :
+  var_id.2 ∉ used_var_names →
+  is_valid_package_name var_id.1 →
+  {{{ own_unused_vars var_id.1 used_var_names }}}
+    globals.put var_id #addr
   {{{ RET #();
-      own_unused_vars_def pkg_name ({[ var_name ]} ∪ used_var_names) ∗
-      is_global_addr_def pkg_name var_name addr
+      own_unused_vars var_id.1 ({[ var_id.2 ]} ∪ used_var_names) ∗
+      is_global_addr var_id addr
   }}}.
 Proof.
-  iIntros (???) "Hpre HΦ".
-  iDestruct "Hpre" as "[#Hinv Hu]".
+  iIntros (???) "Hu HΦ".
   unfold globals.put.
   wp_call_lc "Hlc".
   rewrite to_val_unseal.
   simpl.
+  unseal.
+  iNamed "Hu".
+  unseal.
   iInv "Hinv" as "Hi" "Hclose".
   iMod (lc_fupd_elim_later with "Hlc Hi") as "Hi".
   iNamed "Hi".
-  iNamed "Hu".
   iCombine "Hγpkg Hpkg_gnames" gives %Hlookup.
   iDestruct (big_sepM_delete with "Hglobal_addrs") as "[Hauth2 Hglobal_addrs]".
   { done. }
@@ -113,7 +139,7 @@ Proof.
   iApply (wp_GlobalPut with "[$]").
   iNext.
   iIntros "Hglobals".
-  iMod (ghost_map_insert var_name addr with "Hpkg_auth") as "[Hpkg_auth Hptsto]".
+  iMod (ghost_map_insert var_id.2 addr with "Hpkg_auth") as "[Hpkg_auth Hptsto]".
   { by apply not_elem_of_dom. }
   iMod (ghost_map_elem_persist with "Hptsto") as "#?".
   iDestruct "Hpkg_auth" as "[Hpkg_auth Hpkg_auth2]".
@@ -123,7 +149,7 @@ Proof.
     iFrame.
     iSplitL.
     {
-      iApply (big_sepM_delete _ _ pkg_name).
+      iApply (big_sepM_delete _ _ var_id.1).
       { done. }
       iSplitL "Hpkg_auth".
       - iExists _; iFrame.
@@ -131,7 +157,7 @@ Proof.
         destruct Hg as [Hvalid Hg].
         split; first done.
         intros var_name'.
-        destruct (decide (var_name' = var_name)) as [|Hneq].
+        destruct (decide (var_name' = var_id.2)) as [|Hneq].
         + subst. rewrite !lookup_insert to_val_unseal //.
         + rewrite lookup_insert_ne //.
           rewrite lookup_insert_ne //.
@@ -152,7 +178,7 @@ Proof.
         rewrite -> lookup_insert_ne.
         2:{
           intros Hbad.
-          apply encode_var_name_inj in Hbad as [-> ->]; try assumption.
+          apply encode_var_name_inj in Hbad as [<- <-]; try assumption.
           rewrite lookup_delete_Some in Hlookup'. naive_solver.
         }
         apply Hg.
@@ -169,25 +195,27 @@ Proof.
     rewrite lookup_insert_ne.
     2:{
       intros Hbad.
-      apply encode_var_name_inj in Hbad as [-> ->]; try assumption.
+      apply encode_var_name_inj in Hbad as [<- <-]; try assumption.
       naive_solver.
     }
     naive_solver.
   }
   iApply "HΦ".
+  destruct var_id.
   iFrame "∗#%".
   iPureIntro.
   by rewrite dom_insert_L.
 Qed.
 
-Lemma wp_globals_get pkg_name var_name (addr : loc) :
-  is_valid_package_name pkg_name →
-  {{{ is_globals_inv ∗ is_global_addr_def pkg_name var_name addr }}}
-    globals.get #(encode_var_name pkg_name var_name)
+Lemma wp_globals_get var_id (addr : loc) :
+  is_valid_package_name var_id.1 →
+  {{{ is_global_addr_def var_id addr }}}
+    globals.get var_id #()
   {{{ RET #addr; True }}}.
 Proof.
-  iIntros (??) "Hpre HΦ".
-  iDestruct "Hpre" as "[#Hinv Hu]".
+  iIntros (??) "Hu HΦ".
+  destruct var_id as [pkg_name var_name].
+  iDestruct "Hu" as (?) "(#Hinv & #Hpkg & #Hvar)".
   unfold globals.put.
   wp_call_lc "Hlc".
   rewrite to_val_unseal.
@@ -196,7 +224,6 @@ Proof.
   iInv "Hinv" as "Hi" "Hclose".
   iMod (lc_fupd_elim_later with "Hlc Hi") as "Hi".
   iNamed "Hi".
-  iDestruct "Hu" as (?) "[#Hpkg #Hvar]".
   iCombine "Hpkg Hpkg_gnames" gives %Hlookup.
   iApply (wp_GlobalGet with "[$]").
   iIntros "!> Hglobals".
