new/proof/globals_test.v
@@ -6,17 +6,47 @@ From New.proof Require Import std.
 Section proof.
 
 Context `{!heapGS Σ}.
+Context `{!goGlobalsGS Σ}.
+
+Definition is_defined : iProp Σ :=
+  "HglobalB" ∷ ∃ globalB_addr, is_global_addr globals_test.globalB globalB_addr ∗
+  "HglobalA" ∷ ∃ globalA_addr, is_global_addr globals_test.globalA globalA_addr ∗
+  "HglobalY" ∷ ∃ globalY_addr, is_global_addr globals_test.globalY globalY_addr ∗
+  "HGlobalX" ∷ ∃ GlobalX_addr, is_global_addr globals_test.GlobalX GlobalX_addr
+.
 
 Lemma wp_define' :
-  {{{ True }}}
+  {{{ own_unused_vars globals_test.pkg_name' ∅ }}}
     globals_test.define' #()
-  {{{ RET #(); True }}}.
+  {{{ RET #(); is_defined }}}.
 Proof.
-  iIntros (?) "_ HΦ".
+  iIntros (?) "Hunused HΦ".
   wp_call.
   rewrite -!default_val_eq_zero_val /=.
+
   wp_alloc globalB_ptr as "?".
-Admitted.
+  wp_apply (wp_globals_put with "[Hunused]"); [| | iFrame |]; [set_solver | reflexivity |].
+  iIntros "[Hunused #?]".
+  wp_pures.
+
+  wp_alloc globalA_ptr as "?".
+  wp_apply (wp_globals_put with "[Hunused]"); [| | iFrame |]; [set_solver| reflexivity |].
+  iIntros "[Hunused #?]".
+  wp_pures.
+
+  wp_alloc globalY_ptr as "?".
+  wp_apply (wp_globals_put with "[Hunused]"); [| | iFrame |]; [set_solver| reflexivity |].
+  iIntros "[Hunused #?]".
+  wp_pures.
+
+  wp_alloc GlobalX_ptr as "?".
+  wp_apply (wp_globals_put with "[Hunused]"); [| | iFrame |]; [set_solver| reflexivity |].
+  iIntros "[Hunused #?]".
+  wp_pures.
+
+  iApply "HΦ".
+  iFrame "#".
+Qed.
 
 Lemma wp_initialize' :
   {{{ True }}}
