new/golang/theory.v
@@ -1,6 +1,6 @@
 From Perennial.goose_lang Require Export lang.
 From New.golang Require Export defn.
-From New.golang.theory Require Export exception list typing loop struct mem slice map interface defer typing.
+From New.golang.theory Require Export exception list typing loop struct mem slice map interface defer typing globals.
 
 Export uPred. (* XXX: inherited from proof_prelude.v; not sure why it's here. *)
 Global Set Default Proof Using "Type".
